big fish done

internship_machine.thy
@@ -24,10 +24,13 @@ fun t:: "State \<times> INPUT \<Rightarrow> State \<times> OUT" where
 "t (S_2, n) = (S_2, True)"
 
 
+lemma no_dead_ends: "\<forall>s \<in> \<Sigma>. \<exists>i j. fst(t(s,i)) = j"
+  by auto
+
 
 (*set of all paths*)
 definition paths:: "(nat \<Rightarrow> STEP) set" where
-"paths \<equiv> {p::(nat \<Rightarrow> STEP). STATE(p(0)) = S_1 \<and> (\<forall>n. \<exists>i. t(STATE(p n),i) = (STATE(p(n+1)), OUT(p n)))}"
+"paths \<equiv> {p::(nat \<Rightarrow> STEP). STATE(p(0)) = S_1 \<and> (\<forall>n. \<exists>i. t(STATE(p n),i) = (STATE(p(Suc(n))), OUT(p n)))}"
 
 (*very simple S_1 loop*)
 definition path:: "nat \<Rightarrow> STEP" where
@@ -37,13 +40,43 @@ definition path:: "nat \<Rightarrow> STEP" where
 lemma path_init: "STATE(path(0)) = S_1"
   by (simp add: path_def)
 
+lemma rhs_simp [simp]: " (STATE(path(Suc(n))), OUT(path n)) = (S_1, False)" using path_def by simp
+
+
 lemma path_induct: "(\<forall>n. \<exists>i. t(STATE(path n),i) = (STATE(path(Suc(n))), OUT(path n)))"
+proof (rule allI)
+  fix n
+  have 0: "t(STATE(path n), 0) = (STATE(path(Suc(n))), OUT(path n))" using path_def by simp
+  then show "\<exists>i. t (STATE (path n), i) = (STATE (path (Suc n)), OUT (path n))" using exI by simp
+qed
+
+lemma path_in_paths: "path \<in> paths" using path_induct path_init paths_def
+  by blast
+
+
+lemma "paths \<noteq> {}" using path_in_paths
+  by blast
+
+
+(*check whether there is a path leading between stuffs*)
+inductive route::"nat list \<Rightarrow> State \<Rightarrow> State \<Rightarrow> bool" where
+"fst(t (initial, i)) = current \<Longrightarrow> route [i] initial current"|
+"route [i] initial node \<Longrightarrow> route is node current  \<Longrightarrow> route (i#is) initial current"
+
+(*general path*)
+inductive p::"nat \<Rightarrow> STEP \<Rightarrow> bool" where
+"p 0 \<lparr>INPUT = i, STATE = S_1, OUT = snd(t(S_1, i))\<rparr>"|
+"\<exists>i::nat. p n \<lparr>INPUT = i, STATE = s, OUT = snd(t(s,i))\<rparr> \<Longrightarrow> p (Suc n) \<lparr> INPUT = j, STATE = fst(t(s,i)), OUT = snd(t(fst(t(s,i)), j)) \<rparr>"
+
+lemma big_fish: "\<forall>q\<in>paths. \<forall>m. \<exists>n>m. \<exists>s_0. OUT(q n) = s_0" by auto
+
+
+lemma security: "\<forall>q \<in> paths. \<forall>S \<in> \<Sigma>. \<forall> m. q m = \<lparr>INPUT=1,STATE=S, OUT=True\<rparr>"
 proof
-  fix i
-  let ?case = "n = 0 \<Longrightarrow> \<exists>i. t(STATE(path n),i) = (STATE(path(Suc(n))), OUT(path n))"
-  assume "n = 0"
-  have 1: "t(STATE(path 0), i) = t(S_1,i)" using path_def by simp
-  then have "... = t(S_1, 0)" try
+
+  
+  
+ 
 qed
 
 end
